switch impl to CPS

examples/layeredeffects/LowParseWriters.fst
@@ -25,10 +25,16 @@ module U8 = FStar.UInt8
 module U32 = FStar.UInt32
 module HST = FStar.HyperStack.ST
 
-let read_repr_impl
-  a pre post post_err l spec
-=
-  unit ->
+inline_for_extraction
+let read_repr_impl_direct
+  (a:Type u#x)
+  (pre: pure_pre)
+  (post: pure_post' a pre)
+  (post_err: pure_post_err pre)
+  (l: memory_invariant)
+  (spec: read_repr_spec a pre post post_err)
+: Tot Type0
+= unit ->
   HST.Stack (result a)
   (requires (fun h ->
     B.modifies l.lwrite l.h0 h /\
@@ -37,54 +43,150 @@ let read_repr_impl
   ))
   (ensures (fun h res h' ->
     B.modifies B.loc_none h h' /\
-    res == spec ()
+    begin match spec () with
+      | Correct r -> res == Correct r
+      | Error _ -> Error? res
+    end
   ))
+
+inline_for_extraction
+let read_repr_impl_cps
+  (a:Type u#x)
+  (pre: pure_pre)
+  (post: pure_post' a pre)
+  (post_err: pure_post_err pre)
+  (l: memory_invariant)
+  (spec: read_repr_spec a pre post post_err)
+: Tot Type
+= (h0: HS.mem {B.modifies l.lwrite l.h0 h0 /\ HS.get_tip l.h0 `HS.includes` HS.get_tip h0 }) ->
+  (hpost: (a -> HS.mem -> GTot Type0)) ->
+  (hpost_err: (HS.mem -> GTot Type0)) ->
+  (((r: a) -> HST.Stack unit
+    (requires (fun h ->
+      B.modifies B.loc_none h0 h /\
+      HS.get_tip h0 `HS.includes` HS.get_tip h /\
+      pre /\
+      spec () == Correct r
+    ))
+    (ensures (fun _ _ h -> hpost r h))
+  )) ->
+  ((s: string) -> HST.Stack unit
+    (requires (fun h ->
+      B.modifies B.loc_none h0 h /\
+      HS.get_tip h0 `HS.includes` HS.get_tip h /\
+      pre /\
+      Error? (spec ())
+    ))
+    (ensures (fun _ _ h -> hpost_err h))
+  ) ->
+  HST.Stack unit
+  (requires (fun h ->
+    B.modifies B.loc_none h0 h /\
+    HS.get_tip h0 `HS.includes` HS.get_tip h /\
+    pre
+  ))
+  (ensures (fun _ _ h' ->
+    match spec () with
+    | Correct r -> hpost r h'
+    | _ -> hpost_err h'
+  ))
+
+inline_for_extraction
+let read_repr_impl_direct_to_cps
+  (a:Type u#x)
+  (pre: pure_pre)
+  (post: pure_post' a pre)
+  (post_err: pure_post_err pre)
+  (l: memory_invariant)
+  (spec: read_repr_spec a pre post post_err)
+  (impl: read_repr_impl_direct a pre post post_err l spec)
+: Tot (read_repr_impl_cps a pre post post_err l spec)
+= fun h0 hpost hpost_err k kerr ->
+  match impl () with
+  | Correct r -> k r
+  | Error s -> kerr s
+
+inline_for_extraction
+let read_repr_impl_cps_to_direct
+  (a:Type0)
+  (pre: pure_pre)
+  (post: pure_post' a pre)
+  (post_err: pure_post_err pre)
+  (l: memory_invariant)
+  (spec: read_repr_spec a pre post post_err)
+  (impl: read_repr_impl_cps a pre post post_err l spec)
+: Tot (read_repr_impl_direct a pre post post_err l spec)
+= fun _ ->
+  HST.push_frame ();
+  let bres = B.alloca (Error "read_repr_impl_cps_to_direct" <: result a) 1ul in
+  let h0 = HST.get () in
+  impl
+    h0
+    (fun r h -> B.modifies (B.loc_buffer bres) h0 h /\ Seq.index (B.as_seq h bres) 0 == Correct r)
+    (fun h -> B.modifies (B.loc_buffer bres) h0 h /\ Error? (Seq.index (B.as_seq h bres) 0))
+    (fun r -> B.upd bres 0ul (Correct r))
+    (fun s -> B.upd bres 0ul (Error s))
+  ;
+  let res = B.index bres 0ul in
+  HST.pop_frame ();
+  res
+
+let read_repr_impl
+  a pre post post_err l spec
+=
+  read_repr_impl_cps a pre post post_err l spec
 
 let mk_read_repr_impl
   a pre post post_err l spec impl
 =
-  impl
+  read_repr_impl_direct_to_cps _ _ _ _ _ _ impl
 
 let extract_read_repr_impl
   a pre post post_err l spec impl
 =
-  impl ()
+  read_repr_impl_cps_to_direct _ _ _ _ _ _ impl ()
 
 let read_return_impl
   a x inv
-= fun _ -> Correct x
+= (fun _ _ _ k _ -> k x)
 
 let read_bind_impl
   a b pre_f post_f post_err_f pre_g post_g post_err_g f_bind_impl g l f' g'
 =
-  fun _ ->
-  match f' () with
-  | Correct x -> g' x ()
-  | Error e -> Error e
+  fun h0 kpost kposterr k kerr ->
+    f' h0 
+      (fun x h ->
+        pre_g x /\
+        begin match g x () with | Correct y -> kpost y h | Error s -> kposterr h end
+      )
+      kposterr
+      (fun x -> g' x h0 kpost kposterr k kerr) 
+      kerr
 
 let read_subcomp_impl
   a pre post post_err pre' post' post_err' l l' f_subcomp_spec f_subcomp sq
 =
-  fun _ -> f_subcomp ()
+  fun h0 kpost k kposterr kerr ->
+    f_subcomp h0 kpost k kposterr kerr
 
 let lift_pure_read_impl
   a wp f_pure_spec_for_impl l
 =
-  fun _ -> Correct (f_pure_spec_for_impl ())
+  fun h0 kpost kposterr k kerr -> k (f_pure_spec_for_impl ())
 
 let failwith_impl
   a inv s
-= fun _ -> Error s
+= fun h0 kpost k kposterr kerr -> kerr s
 
 let buffer_index_impl
   #t inv b i
 =
-  fun _ -> Correct (B.index b i)
+  fun h0 kpost kposterr k kerr -> k (B.index b i)
 
 let buffer_sub_impl
   #t inv b i len
 =
-  fun _ -> Correct (B.sub b i len)
+  fun h0 kpost kposterr k kerr -> k (B.sub b i len)
 
 noeq
 type rptr = {
@@ -120,11 +222,12 @@ let valid_rptr_frame
 = valid_frame p inv.h0 x.rptr_base 0ul (B.len x.rptr_base) inv.lwrite inv'.h0
 
 let deref_impl
-  #p #inv r x _
+  #p #inv r x
+  h0 kpost kposterr k kerr
 =
   let h = HST.get () in
   valid_frame p inv.h0 x.rptr_base 0ul (B.len x.rptr_base) inv.lwrite h;
-  Correct (r x.rptr_base x.rptr_len)
+  k (r x.rptr_base x.rptr_len)
 
 let access_spec
   #p1 #p2 #lens #inv g x
@@ -134,15 +237,15 @@ let access_spec
 
 let access_impl
   #p1 #p2 #lens #inv #g a x
+  h0 kpost kposterr k kerr
 =
-  fun _ ->
   let h = HST.get () in
   valid_frame p1 inv.h0 x.rptr_base 0ul (B.len x.rptr_base) inv.lwrite h;
   let (base', len') = baccess a x.rptr_base x.rptr_len in
   let h' = HST.get () in
   gaccessor_frame g inv.h0 x.rptr_base inv.lwrite h;
   gaccessor_frame g inv.h0 x.rptr_base inv.lwrite h';
-  Correct ({ rptr_base = base'; rptr_len = len' })
+  k ({ rptr_base = base'; rptr_len = len' })
 
 let validate_spec
   p inv b
@@ -177,7 +280,8 @@ let valid_frame'
 
 let validate_impl
   #p v inv b len
-= fun _ ->
+  h0 kpost kposterr k kerr
+=
   let h1 = HST.get () in
   Classical.forall_intro (valid_frame' p inv.h0 b 0ul inv.lwrite h1);
   gvalidate_frame p inv.h0 b inv.lwrite h1;
@@ -186,13 +290,14 @@ let validate_impl
   Classical.forall_intro (valid_frame' p inv.h0 b 0ul inv.lwrite h2);
   gvalidate_frame p inv.h0 b inv.lwrite h2;
   match res with
-  | None -> Error "validation failed"
+  | None -> kerr "validation failed"
   | Some pos ->
     let b' = B.sub b 0ul pos in
     let x = { rptr_base = b' ; rptr_len = pos } in
-    Correct (x, pos)
+    k (x, pos)
 
-let repr_impl
+inline_for_extraction
+let repr_impl_direct
   (a:Type u#x)
   (r_in: parser)
   (r_out: parser)
@@ -216,35 +321,204 @@ let repr_impl
     repr_impl_post a r_in r_out pre post post_err l spec b pos1 h res h'
   ))
 
+inline_for_extraction
+let repr_impl_cps
+  (a:Type u#x)
+  (r_in: parser)
+  (r_out: parser)
+  (pre: pre_t r_in)
+  (post: post_t a r_in r_out pre)
+  (post_err: post_err_t r_in pre)
+  (l: memory_invariant)
+  (spec: repr_spec a r_in r_out pre post post_err)
+: Tot Type =
+  (b: B.buffer u8 { l.lwrite `B.loc_includes` B.loc_buffer b }) ->
+  (len: U32.t { len == B.len b }) ->
+  (pos1: buffer_offset b) ->
+  (h0: HS.mem {
+    B.modifies l.lwrite l.h0 h0 /\
+    HS.get_tip l.h0 `HS.includes` HS.get_tip h0 /\
+    valid_pos r_in h0 b 0ul pos1 /\
+    pre (contents r_in h0 b 0ul pos1)
+  }) ->
+  (hpost: (a -> Parser?.t r_out -> HS.mem -> GTot Type0)) ->
+  (((r: a) -> (pos2: buffer_offset b) -> HST.Stack unit
+    (requires (fun h ->
+      HS.get_tip h0 `HS.includes` HS.get_tip h /\
+      B.modifies (B.loc_buffer b) h0 h /\
+      U32.v pos1 <= U32.v pos2 /\
+      valid_pos r_out h b 0ul pos2 /\
+      spec (contents r_in h0 b 0ul pos1) == Correct (r, contents r_out h b 0ul pos2)
+    ))
+    (ensures (fun h _ h' ->
+      hpost r (contents r_out h b 0ul pos2) h'
+    ))
+  )) ->
+  (hpost_overflow: (HS.mem -> GTot Type0)) ->
+  (unit -> HST.Stack unit
+    (requires (fun h ->
+      HS.get_tip h0 `HS.includes` HS.get_tip h /\
+      B.modifies (B.loc_buffer b) h0 h /\
+      begin match spec (contents r_in h0 b 0ul pos1) with
+      | Correct (r, v') -> size r_out v' > B.length b
+      | _ -> True
+      end
+    ))
+    (ensures (fun _ _ h -> hpost_overflow h))
+  ) ->
+  (hpost_err: (HS.mem -> GTot Type0)) ->
+  ((s: string) -> HST.Stack unit
+    (requires (fun h ->
+      HS.get_tip h0 `HS.includes` HS.get_tip h /\
+      B.modifies (B.loc_buffer b) h0 h /\
+      Error? (spec (contents r_in h0 b 0ul pos1))
+    ))
+    (ensures (fun _ _ h -> hpost_err h))
+  ) ->
+  HST.Stack unit
+  (requires (fun h ->
+    B.modifies B.loc_none h0 h /\
+    HS.get_tip h0 `HS.includes` HS.get_tip h
+  ))
+  (ensures (fun _ _ h' ->
+    match spec (contents r_in h0 b 0ul pos1) with
+    | Correct (r, v') ->
+      if size r_out v' > B.length b
+      then hpost_overflow h'
+      else hpost r v' h'
+    | _ -> hpost_overflow h' \/ hpost_err h'
+  ))
+
+inline_for_extraction
+let repr_impl_direct_to_cps
+  (a:Type u#x)
+  (r_in: parser)
+  (r_out: parser)
+  (pre: pre_t r_in)
+  (post: post_t a r_in r_out pre)
+  (post_err: post_err_t r_in pre)
+  (l: memory_invariant)
+  (spec: repr_spec a r_in r_out pre post post_err)
+  (impl: repr_impl_direct a r_in r_out pre post post_err l spec)
+: Tot (repr_impl_cps a r_in r_out pre post post_err l spec)
+=
+  fun b len pos1 
+  h0 hpost k hpost_overflow koverflow hpost_err kerr ->
+  let h = HST.get () in
+  valid_frame r_in h0 b 0ul pos1 B.loc_none h;
+  match impl b len pos1 with
+  | ICorrect v pos2 -> k v pos2
+  | IOverflow -> koverflow ()
+  | IError s -> kerr s
+
+inline_for_extraction
+let repr_impl_cps_to_direct
+  (a:Type0)
+  (r_in: parser)
+  (r_out: parser)
+  (pre: pre_t r_in)
+  (post: post_t a r_in r_out pre)
+  (post_err: post_err_t r_in pre)
+  (l: memory_invariant)
+  (spec: repr_spec a r_in r_out pre post post_err)
+  (impl: repr_impl_cps a r_in r_out pre post post_err l spec)
+: Tot (repr_impl_direct a r_in r_out pre post post_err l spec)
+=
+  fun b len pos1 ->
+  let h0 = HST.get () in
+  HST.push_frame ();
+  let bres = B.alloca (IError "repr_impl_cps_to_direct" <: iresult a) 1ul in
+  let h1 = HST.get () in
+  valid_frame r_in h0 b 0ul pos1 B.loc_none h1;
+  impl
+    b len pos1
+    h1
+    (fun r v' h ->
+      B.modifies (B.loc_buffer b `B.loc_union` B.loc_buffer bres) h1 h /\
+      begin match Seq.index (B.as_seq h bres) 0 with
+      | ICorrect r' pos2 ->
+        r == r' /\
+        valid_pos r_out h b 0ul pos2 /\
+        contents r_out h b 0ul pos2 == v'
+      | _ -> False
+      end
+    )
+    (fun r pos2 ->
+      let h2 = HST.get () in
+      B.upd bres 0ul (ICorrect r pos2);
+      let h = HST.get () in
+      valid_frame r_out h2 b 0ul pos2 (B.loc_buffer bres) h
+    )
+    (fun h -> B.modifies (B.loc_buffer b `B.loc_union` B.loc_buffer bres) h1 h /\ IOverflow? (Seq.index (B.as_seq h bres) 0))
+    (fun s -> B.upd bres 0ul IOverflow)
+    (fun h -> B.modifies (B.loc_buffer b `B.loc_union` B.loc_buffer bres) h1 h /\ IError? (Seq.index (B.as_seq h bres) 0))
+    (fun s -> B.upd bres 0ul (IError s))
+  ;
+  let h3 = HST.get () in
+  let res = B.index bres 0ul in
+  HST.pop_frame ();
+  let h4 = HST.get () in
+  let f (pos2: U32.t) : Lemma
+    (requires (valid_pos r_out h3 b 0ul pos2))
+    (ensures (
+      valid_pos r_out h3 b 0ul pos2 /\
+      valid_pos r_out h4 b 0ul pos2 /\
+      contents r_out h4 b 0ul pos2 == contents r_out h3 b 0ul pos2
+    ))
+  =
+    valid_frame r_out h3 b 0ul pos2 (B.loc_all_regions_from false (HS.get_tip h1)) h4
+  in
+  Classical.forall_intro (Classical.move_requires f);
+  res
+
+let repr_impl = repr_impl_cps
+
 let mk_repr_impl
   a r_in r_out pre post post_err l spec impl
 =
-  impl
+  repr_impl_direct_to_cps _ _ _ _ _ _ _ _ impl
 
 let extract_repr_impl
   a r_in r_out pre post post_err l spec impl
 =
-  impl
+  repr_impl_cps_to_direct _ _ _ _ _ _ _ _ impl
 
 inline_for_extraction
 let return_impl
   a x r l
-= fun b len pos1 -> ICorrect x pos1
+= fun b len pos1 
+  h0 hpost k hpost_overflow koverflow hpost_err kerr ->
+  let h = HST.get () in
+  valid_frame r h0 b 0ul pos1 B.loc_none h;
+  k x pos1
 
 inline_for_extraction
 let bind_impl
   a b r_in_f r_out_f pre_f post_f post_err_f r_out_g pre_g post_g post_err_g f_bind_impl g l f' g'
-= fun buf len pos ->
-  match f' buf len pos with
-  | IError e -> IError e
-  | IOverflow -> IOverflow
-  | ICorrect x posf -> g' x buf len posf
+= fun buf len pos 
+  h0 hpost k hpost_overflow koverflow hpost_err kerr ->
+  f' buf len pos h0
+    (fun x vg h' ->
+      pre_g x vg /\
+      begin match g x vg with
+      | Correct (y, v') ->
+        if size r_out_g v' > B.length buf
+        then hpost_overflow h'
+        else hpost y v' h'
+      | Error s -> hpost_overflow h' \/ hpost_err h'
+      end
+    )
+    (fun x posf -> let h1 = HST.get () in g' x buf len posf h1 hpost k hpost_overflow koverflow hpost_err kerr)
+    hpost_overflow koverflow
+    hpost_err kerr
 
 inline_for_extraction
 let subcomp_impl
   a r_in r_out pre post post_err pre' post' post_err' l l' f_subcomp_spec f_subcomp sq
 : Tot (repr_impl a r_in r_out pre' post' post_err' l' (subcomp_spec a r_in r_out pre post post_err pre' post' post_err' f_subcomp_spec))
-= (fun b len pos -> f_subcomp b len pos)
+= fun b len pos
+  h0 hpost k hpost_overflow koverflow hpost_err kerr ->
+  f_subcomp b len pos h0 hpost k hpost_overflow koverflow hpost_err kerr
 
 (*
 inline_for_extraction
@@ -257,29 +531,40 @@ let lift_pure_impl
 
 let lift_read_impl
   a pre post post_err inv r f_read_spec
-=
-  fun b len pos ->
-    let h = HST.get () in
-    match ReadRepr?.impl f_read_spec () with
-    | Correct res -> 
+= fun b len pos
+  h0 hpost k hpost_overflow koverflow hpost_err kerr ->
+  let h = HST.get () in
+  valid_frame r h0 b 0ul pos B.loc_none h;
+  ReadRepr?.impl f_read_spec
+    h
+    (fun a h' -> hpost a (contents r h0 b 0ul pos) h')
+    hpost_err
+    (fun res ->
       let h' = HST.get () in
       valid_frame r h b 0ul pos B.loc_none h';
-      ICorrect res pos
-    | Error e ->
-      IError e
+      k res pos
+    )
+    (fun s -> kerr s)
 
 let wfailwith_impl
   a inv rin rout s
 =
-  fun b len pos ->
-  IError s
+  fun b len pos
+  h0 hpost k hpost_overflow koverflow hpost_err kerr ->
+  kerr s
 
 let get_state_impl
   inv p
 =
-  fun b len pos ->
+  fun b len pos
+    h0 hpost k hpost_overflow koverflow hpost_err kerr ->
     let h = HST.get () in
-    ICorrect (Ghost.hide (contents p h b 0ul pos)) pos
+    valid_frame p h0 b 0ul pos B.loc_none h;
+    k (Ghost.hide (contents p h b 0ul pos)) pos
+
+#push-options "--ifuel 8"
+
+#restart-solver
 
 inline_for_extraction
 let frame_impl
@@ -292,30 +577,37 @@ let frame_impl
   (l: memory_invariant)
   (inner: unit -> EWrite a parse_empty p pre post post_err l)
 : Tot (repr_impl a frame (frame_out a frame p) (frame_pre frame pre) (frame_post a frame pre p post) (frame_post_err frame pre post_err) l (frame_spec a frame pre p post post_err l inner))
-= fun buf len pos ->
+= fun buf len pos
+    h0 hpost k hpost_overflow koverflow hpost_err kerr ->
   let h = HST.get () in
+  valid_frame frame h0 buf 0ul pos B.loc_none h;
   let buf' = B.offset buf pos in
-  match destr_repr_impl a parse_empty p pre post post_err l inner buf' (len `U32.sub` pos) 0ul with
-  | IError e -> IError e
-  | IOverflow -> IOverflow
-  | ICorrect x wlen ->
-    let h' = HST.get () in
-    let pos' = pos `U32.add` wlen in
-    B.loc_disjoint_loc_buffer_from_to buf 0ul pos pos (B.len buf');
-    valid_frame frame h buf 0ul pos (B.loc_buffer buf') h';
-    valid_parse_pair frame (p) h' buf 0ul pos pos' ;
-    ICorrect x pos'
+  destr_repr_impl a parse_empty p pre post post_err l inner buf' (len `U32.sub` pos) 0ul
+    h 
+    (fun x v' h' -> hpost x (contents frame h0 buf 0ul pos, v') h')
+    (fun x wlen ->
+      let h' = HST.get () in
+      let pos' = pos `U32.add` wlen in
+      B.loc_disjoint_loc_buffer_from_to buf 0ul pos pos (B.len buf');
+      valid_frame frame h buf 0ul pos (B.loc_buffer buf') h';
+      valid_parse_pair frame (p) h' buf 0ul pos pos' ;
+      k x pos' )
+    hpost_overflow koverflow
+    hpost_err kerr
+
+#pop-options
 
 #push-options "--z3rlimit 128"
 
 let elem_writer_impl
   #p w l x
 =
-  fun b len pos ->
+  fun b len pos
+    h0 hpost k hpost_overflow koverflow hpost_err kerr ->
   let b' = B.offset b pos in
   match w b' (len `U32.sub` pos) x with
-  | None -> IOverflow
-  | Some xlen -> ICorrect () (pos `U32.add` xlen)
+  | None -> koverflow ()
+  | Some xlen -> k () (pos `U32.add` xlen)
 
 inline_for_extraction
 let recast_writer_impl
@@ -337,25 +629,30 @@ let recast_writer_impl
 inline_for_extraction
 let frame2_impl
   a frame ppre pre p post post_err l inner
-= fun buf len pos ->
+= fun buf len pos
+    h0 hpost k hpost_overflow koverflow hpost_err kerr ->
   let h = HST.get () in
+  valid_frame (frame `parse_pair` ppre) h0 buf 0ul pos B.loc_none h;
   let pos2 = valid_parse_pair_inv frame ppre buf len 0ul pos in
   let buf' = B.offset buf pos2 in
   assert (valid_pos ppre h buf pos2 pos);
   assert (valid_pos ppre h buf' 0ul (pos `U32.sub` pos2));
   let h1 = HST.get () in
+  valid_frame frame h buf 0ul pos2 B.loc_none h1;
   valid_frame ppre h buf' 0ul (pos `U32.sub` pos2) B.loc_none h1;
-  match destr_repr_impl a ppre p pre post post_err l inner buf' (len `U32.sub` pos2) (pos `U32.sub` pos2) with
-  | IOverflow ->
-    IOverflow
-  | IError e -> IError e
-  | ICorrect x wlen ->
-    let h' = HST.get () in
-    let pos' = pos2 `U32.add` wlen in
-    B.loc_disjoint_loc_buffer_from_to buf 0ul pos2 pos2 (B.len buf');
-    valid_frame frame h buf 0ul pos2 (B.loc_buffer buf') h';
-    valid_parse_pair frame (p) h' buf 0ul pos2 pos' ;
-    ICorrect x pos'
+  destr_repr_impl a ppre p pre post post_err l inner buf' (len `U32.sub` pos2) (pos `U32.sub` pos2)
+    h1
+    (fun x v' h' -> hpost x (contents frame h buf 0ul pos2, v') h')
+    (fun x wlen ->
+      let h' = HST.get () in
+      let pos' = pos2 `U32.add` wlen in
+      B.loc_disjoint_loc_buffer_from_to buf 0ul pos2 pos2 (B.len buf');
+      valid_frame frame h buf 0ul pos2 (B.loc_buffer buf') h';
+      valid_parse_pair frame (p) h' buf 0ul pos2 pos' ;
+      k x pos'
+    )
+    hpost_overflow koverflow
+    hpost_err kerr
 
 #pop-options
 
@@ -364,10 +661,12 @@ let frame2_impl
 let valid_rewrite_impl
   p1 p2 precond f v inv
 =
-  fun buf len pos ->
+  fun buf len pos
+    h0 hpost k hpost_overflow koverflow hpost_err kerr ->
     let h = HST.get () in
+    valid_frame p1 h0 buf 0ul pos B.loc_none h;
     v.valid_rewrite_valid h buf 0ul pos;
-    ICorrect () pos
+    k () pos
 
 let cast
   p1 p2 precond f v inv x1
@@ -391,14 +690,16 @@ let check_precond_impl
   (c: check_precond_t p1 precond)
   (inv: memory_invariant)
 : Tot (repr_impl unit p1 (p1) precond (fun vin _ vout -> vin == vout /\ precond vin) (fun vin -> ~ (precond vin)) inv (check_precond_spec p1 precond))
-= fun b len pos ->
+= fun b len pos
+    h0 hpost k hpost_overflow koverflow hpost_err kerr ->
   let h = HST.get () in
+  valid_frame p1 h0 b 0ul pos B.loc_none h;
   if c b len 0ul pos
   then
     let h' = HST.get () in
     let _ = valid_frame p1 h b 0ul pos B.loc_none h' in
-    ICorrect () pos
-  else IError "check_precond failed"
+    k () pos
+  else kerr "check_precond failed"
 
 let check_precond_repr
   p1 precond c inv
@@ -407,13 +708,14 @@ let check_precond_repr
 let cat_impl
   #inv #p x
 =
-  fun b len _ ->
+  fun b len _
+    h0 hpost k hpost_overflow koverflow hpost_err kerr ->
   if len `U32.lt` x.rptr_len
   then
-    IOverflow
+    koverflow ()
   else begin
     B.blit x.rptr_base 0ul b 0ul x.rptr_len;
     let h' = HST.get () in
     valid_ext p inv.h0 x.rptr_base 0ul x.rptr_len h' b 0ul x.rptr_len;
-    ICorrect () x.rptr_len
+    k () x.rptr_len
   end
